Comment out wrong proof of block_membership_property_is_majority_driven (#39)

Isabelle/TFGCasper.thy
@@ -30,22 +30,22 @@ notation (ASCII)
   comp  (infixl "blockchain_membership" 70)
 
 (* Definition 4.27: Score of a block *)
-fun (in GhostParams) score :: "state \<Rightarrow> block \<Rightarrow> real"
+definition (in GhostParams) score :: "state \<Rightarrow> block \<Rightarrow> real"
   where
     "score \<sigma> b = sum W {v \<in> observed \<sigma>. \<exists> b' \<in> B. b' \<in> (latest_estimates_from_non_equivocating_validators \<sigma> v) \<and> (b \<downharpoonright> b')}"
 
 (* Definition 4.28: Children *)
-fun (in GhostParams) children :: "block * state \<Rightarrow> block set"
+definition (in GhostParams) children :: "block * state \<Rightarrow> block set"
   where
-    "children (b, \<sigma>) = {b' \<in> est `\<sigma>. b = prev b'}"
+    "children = (\<lambda>(b, \<sigma>). {b' \<in> est `\<sigma>. b = prev b'})"
 
 (* Definition 4.29: Best Children *)
-fun (in GhostParams) best_children :: "block * state \<Rightarrow>  block set"
+definition (in GhostParams) best_children :: "block * state \<Rightarrow>  block set"
   where
-    "best_children (b, \<sigma>) = {arg_max_on (score \<sigma>) (children (b, \<sigma>))}"
+    "best_children = (\<lambda> (b, \<sigma>). {arg_max_on (score \<sigma>) (children (b, \<sigma>))})"
 
 (* Definition 4.30: GHOST *)
-(* Question3: well-ortedness error *)
+(* NOTE: well-sortedness error occurs in code generation *)
 function (in GhostParams) GHOST :: "(block set * state) => block set"
   where
     "GHOST (b_set, \<sigma>) =
@@ -54,41 +54,52 @@ function (in GhostParams) GHOST :: "(block set * state) => block set"
   by auto
 
 (* Definition 4.31: Casper the Friendly Ghost *)
-fun (in GhostParams) estimator :: "state \<Rightarrow> block set"
+definition (in GhostParams) GHOST_estimator :: "state \<Rightarrow> block set"
   where
-    "estimator \<sigma> = GHOST ({genesis}, \<sigma>)"
+    "GHOST_estimator \<sigma> = GHOST ({genesis}, \<sigma>) \<union> (\<Union> b \<in> GHOST ({genesis}, \<sigma>). children (b, \<sigma>))"
 
 (* Definition 4.32: Example non-trivial properties of consensus values *)
 abbreviation (in GhostParams) P :: "consensus_value_property set"
   where
     "P \<equiv> {p. \<exists>!b \<in> B. \<forall>b' \<in> B. (b \<downharpoonright> b' \<longrightarrow> p b' = True) \<and> \<not> (b \<downharpoonright> b' \<longrightarrow> p b' = False)}"
 
-
-lemma (in GhostParams) GHOST_is_valid_estimator : 
-  "(\<forall> b. b \<in> B \<longleftrightarrow> prev b \<in> B) \<and> B = C \<and> genesis \<in> C 
-  \<Longrightarrow> is_valid_estimator estimator"
-  apply simp
-  oops
-
 (* Locale for proofs *)
 locale Ghost = GhostParams + Protocol +
   assumes prev_type : "\<forall> b. b \<in> B \<longleftrightarrow> prev b \<in> B"
   and block_is_consensus_value : "B = C"
-  and ghost_is_estimator : "\<epsilon> = estimator"
+  and ghost_is_estimator : "\<epsilon> = GHOST_estimator"
   and genesis_type : "genesis \<in> C"
 
 lemma (in Ghost) children_type :
   "\<forall> b \<sigma>. b \<in> B \<and> \<sigma> \<in> \<Sigma> \<longrightarrow>  children (b, \<sigma>) \<subseteq> B"
+  apply (simp add: children_def)
   using Ghost_axioms Ghost_axioms_def Ghost_def by auto
+
+lemma (in Ghost) best_children_type :
+  "\<forall> b \<sigma>. b \<in> B \<and> \<sigma> \<in> \<Sigma> \<longrightarrow>  best_children (b, \<sigma>) \<subseteq> B"
+  apply (simp add: best_children_def arg_max_on_def arg_max_def is_arg_max_def)
+  apply auto 
+  oops
+
+lemma (in Ghost) GHSOT_type :
+  "\<forall> \<sigma> b_set. \<sigma> \<in> \<Sigma> \<and> b_set \<subseteq> B \<longrightarrow>  GHOST(b_set, \<sigma>) \<subseteq> B"
+  oops
+
+lemma (in GhostParams) GHOST_is_valid_estimator : 
+  "(\<forall> b. b \<in> B \<longleftrightarrow> prev b \<in> B) \<and> B = C \<and> genesis \<in> C 
+  \<Longrightarrow> is_valid_estimator GHOST_estimator"
+  apply (simp add: is_valid_estimator_def GhostParams.GHOST_estimator_def)
+  oops
 
 lemma (in Ghost) block_membership_property_is_majority_driven :
   "\<forall> p \<in> P. is_majority_driven p"
-  apply simp
-  by (metis DiffE Pow_iff is_valid_estimator_def \<epsilon>_type block_is_consensus_value is_majority_driven_def subsetCE)
+  apply (simp add: is_majority_driven_def)
+  (* by (metis DiffE Pow_iff is_valid_estimator_def \<epsilon>_type block_is_consensus_value subsetCE) *)
+  oops
 
 lemma (in Ghost) block_membership_property_is_max_driven :
   "\<forall> p \<in> P. is_max_driven p"
-  apply simp
+  apply (simp add: is_max_driven_def)
   (* FIXME: Timeout *)
   (* by (metis DiffE Nats_0 ghost_is_estimator) *)
   oops
